Core/Program.v
@@ -15,30 +15,30 @@ Instance coerceSumRight S E F `{SigCoercion S F} : SigCoercion S (Sum E F) :=
   fun _ s => inr (coerceOp _ s).
 
 CoInductive Prog {E : ESig} {B : Type} : Type :=
-| Bind {A} : E A -> (A -> Prog) -> Prog
+| Vis {A} : E A -> (A -> Prog) -> Prog
 | Return : B -> Prog
-| NoOp : Prog -> Prog.
+| Tau : Prog -> Prog.
 Arguments Prog : clear implicits.
 Arguments Return {E A} : rename.
-Arguments NoOp {E A} : rename.
+Arguments Tau {E A} : rename.
 
-Definition Impl {E : ESig} {F : ESig} := (forall Ret, F Ret -> Prog E Ret).
+Definition Impl {E : ESig} {F : ESig} := (forall R, F R -> Prog E R).
 Arguments Impl : clear implicits.
 
 (* Identity Program and Implementation *)
-Definition idProg {E : ESig} {Ret : Type} : E Ret -> Prog E Ret := 
-    fun e => (Bind e Return).
+Definition idProg {E : ESig} {R : Type} : E R -> Prog E R := 
+    fun e => (Vis e Return).
 
 Definition idImpl {E : ESig} : Impl E E := 
-    fun Ret => idProg.
+    fun _ => idProg.
 
 (* Program Operations *)
 
 CoFixpoint bindProg {E A B} (p : Prog E A) (f : A -> Prog E B) : Prog E B :=
   match p with
-    | Bind e f' => Bind e (fun x => bindProg (f' x) f)
+    | Vis e f' => Vis e (fun x => bindProg (f' x) f)
     | Return a => f a
-    | NoOp p' => NoOp (bindProg p' f)
+    | Tau p' => Tau (bindProg p' f)
   end.
 Notation "x <- f ; m" := (bindProg f (fun x => m)) (at level 80, right associativity).
 Notation "f ;; m" := (bindProg f (fun _ => m)) (at level 80, right associativity).
@@ -46,58 +46,58 @@ Notation "f ;; m" := (bindProg f (fun _ => m)) (at level 80, right associativity
 CoFixpoint mapProg
            {E E'}
            (f : forall A, E A -> E' A)
-           {Ret}
-           (p : Prog E Ret) :
-  Prog E' Ret :=
+           {R}
+           (p : Prog E R) :
+  Prog E' R :=
   match p with
-    | Bind e f' => Bind (f _ e) (fun a => mapProg f (f' a))
+    | Vis e f' => Vis (f _ e) (fun a => mapProg f (f' a))
     | Return r => Return r
-    | NoOp p' => NoOp (mapProg f p')
+    | Tau p' => Tau (mapProg f p')
   end.
 
 CoFixpoint substProg
            {E F}
            (impl : Impl E F)
-           {Ret}
-           (p : Prog F Ret) :
-  Prog E Ret :=
+           {R}
+           (p : Prog F R) :
+  Prog E R :=
   match p with
-    | Bind m f => NoOp (bindSubstProg impl f (impl _ m))
+    | Vis m f => Tau (bindSubstProg impl f (impl _ m))
     | Return a => Return a
-    | NoOp p' => NoOp (substProg impl p')
+    | Tau p' => Tau (substProg impl p')
   end
 
 with bindSubstProg
            {F F'} (impl : forall A, F' A -> Prog F A)
            {R R'} (f: R -> Prog F' R') (p: Prog F R) :=
   match p with
-  | Bind m' f' => Bind m' (fun r => bindSubstProg impl f (f' r))
-  | Return a => NoOp (substProg impl (f a))
-  | NoOp p'' => NoOp (bindSubstProg impl f p'')
+  | Vis m' f' => Vis m' (fun r => bindSubstProg impl f (f' r))
+  | Return a => Tau (substProg impl (f a))
+  | Tau p'' => Tau (bindSubstProg impl f p'')
   end.
 
 Definition implVComp {E F G} (impl : Impl E F) (impl' : Impl F G) : Impl E G := 
-    fun Ret g => substProg impl (impl' Ret g).
+    fun _ g => substProg impl (impl' _ g).
 
 Notation "x |> y" := (implVComp x y) (at level 80, right associativity).
 
-CoInductive progEq {E} {Ret}: Prog E Ret -> Prog E Ret -> Prop :=
-| BindEq Ret' (e: E Ret') (f1: Ret' -> Prog E Ret) (f2: Ret' -> Prog E Ret):
+CoInductive progEq {E} {R}: Prog E R -> Prog E R -> Prop :=
+| VisEq R' (e: E R') (f1: R' -> Prog E R) (f2: R' -> Prog E R):
     (forall v, progEq (f1 v) (f2 v)) ->
-    progEq (Bind e f1) (Bind e f2)
+    progEq (Vis e f1) (Vis e f2)
 | ReturnEq r:
     progEq (Return r) (Return r)
 | NoopEq p1 p2:
     progEq p1 p2 ->
-    progEq (NoOp p1) (NoOp p2).
+    progEq (Tau p1) (Tau p2).
 
 Definition implEq {E F} (impl : Impl E F) (impl' : Impl E F) : Prop :=
-  forall Ret (f : F Ret), progEq (impl Ret f) (impl' Ret f).
+  forall R (f : F R), progEq (impl R f) (impl' R f).
 
 (* Control/extra constructs *)
 
 Definition call {E F A} `{SigCoercion E F} (m : E A) : Prog F A :=
-  Bind (coerceOp A m) Return.
+  Vis (coerceOp A m) Return.
 
 Definition ret {E A} := @Return E A.
 
@@ -109,12 +109,12 @@ Context {E} (t : Prog E bool) (e : Prog E unit).
 
 CoFixpoint whileAux (t' : Prog E bool) (e' : Prog E unit) : Prog E unit :=
   match t', e' with
-  | Bind m k, e' => Bind m (fun x => whileAux (k x) e')
-  | NoOp t', e' => NoOp (whileAux t' e')
+  | Vis m k, e' => Vis m (fun x => whileAux (k x) e')
+  | Tau t', e' => Tau (whileAux t' e')
   | Return false, _ => skip
-  | Return true, Bind m k => Bind m (fun x => whileAux (Return true) (k x))
-  | Return true, NoOp e' => NoOp (whileAux (Return true) e')
-  | Return true, Return _ => NoOp (whileAux t e)
+  | Return true, Vis m k => Vis m (fun x => whileAux (Return true) (k x))
+  | Return true, Tau e' => Tau (whileAux (Return true) e')
+  | Return true, Return _ => Tau (whileAux t e)
   end.
 
 Definition while := whileAux t e.
@@ -133,9 +133,9 @@ Context {E A} (e : Prog E (ControlFlow A)).
 CoFixpoint loopAux (e' : Prog E (ControlFlow A)) : Prog E A :=
   match e' with
   | Return (Break v) => Return v
-  | Return Continue => NoOp (loopAux e)
-  | NoOp e' => NoOp (loopAux e')
-  | Bind m k => Bind m (fun x => loopAux (k x))
+  | Return Continue => Tau (loopAux e)
+  | Tau e' => Tau (loopAux e')
+  | Vis m k => Vis m (fun x => loopAux (k x))
   end.
 
 Definition loop := loopAux e.
